ulib/experimental/Steel.HigherArray0.fsti
@@ -1,0 +1,268 @@
+module Steel.HigherArray0
+
+module P = Steel.FractionalPermission
+module U32 = FStar.UInt32
+
+open Steel.Memory
+open Steel.Effect.Atomic
+open Steel.Effect
+
+/// NOTE: This module is slated to have primitive Karamel extraction
+/// (except for definitions meant to be inlined.)
+
+/// An abstract type to represent a base array (whole allocation
+/// unit), exposed for proof purposes only
+[@@erasable]
+val base_t (elt: Type u#a) : Tot Type0
+val base_len (#elt: Type) (b: base_t elt) : GTot nat
+
+/// An abstract type to represent a C pointer, as a base and an offset
+/// into its base
+[@@noextract_to "krml"] // primitive
+val ptr (elt: Type u#a) : Type0
+val base (#elt: Type) (p: ptr elt) : Tot (base_t elt)
+val offset (#elt: Type) (p: ptr elt) : Ghost nat (requires True) (ensures (fun offset -> offset <= base_len (base p)))
+val ptr_base_offset_inj (#elt: Type) (p1 p2: ptr elt) : Lemma
+  (requires (
+    base p1 == base p2 /\
+    offset p1 == offset p2
+  ))
+  (ensures (
+    p1 == p2
+  ))
+
+/// A concrete type to represent a C array, as a C pointer and a ghost
+/// array length.  By virtue of the length being ghost, Karamel will
+/// extract this type as just ptr, but to inline the definition of
+/// this type, we use standard dependent pairs instead of a custom
+/// record type.
+inline_for_extraction
+[@@noextract_to "krml"]
+let array (elt: Type u#a) : Tot Type0 =
+  (p: ptr elt & (length: Ghost.erased nat {offset p + length <= base_len (base p)}))
+
+/// This will extract to "let p = a"
+inline_for_extraction
+[@@noextract_to "krml"]
+let ptr_of
+  (#elt: Type)
+  (a: array elt)
+: Tot (ptr elt)
+= match a with // dfst is not marked inline_for_extraction, so we need to reimplement it
+  | (| p, _ |) -> p
+
+let length (#elt: Type) (a: array elt) : GTot nat =
+  dsnd a
+
+/// A Steel separation logic heap predicate to describe that an array
+/// a points to some element sequence s with some permission p.
+/// vprop limits the universe to at most 1 (because of the selector,
+/// although the latter is not used here)
+val pts_to
+  (#elt: Type u#1) (a: array elt)
+  ([@@@ smt_fallback ] p: P.perm)
+  ([@@@ smt_fallback ] s: Seq.seq elt)
+: Tot vprop
+
+/// Allocating a new array of size n, where each cell is initialized
+/// with value x
+[@@noextract_to "krml"] // primitive
+val alloc
+  (#elt: Type)
+  (x: elt)
+  (n: U32.t)
+: Steel (array elt)
+    emp
+    (fun a -> pts_to a P.full_perm (Seq.create (U32.v n) x))
+    (fun _ -> True)
+    (fun _ a _ -> length a == U32.v n)
+
+/// Sharing and gathering permissions on an array. Those only
+/// manipulate permissions, so they are nothing more than stateful
+/// lemmas.
+val share
+  (#opened: _)
+  (#elt: Type)
+  (#x: Seq.seq elt)
+  (a: array elt)
+  (p p1 p2: P.perm)
+: SteelGhost unit opened
+    (pts_to a p x)
+    (fun _ -> pts_to a p1 x `star` pts_to a p2 x)
+    (fun _ -> p == p1 `P.sum_perm` p2)
+    (fun _ _ _ -> True)
+
+val gather
+  (#opened: _)
+  (#elt: Type)
+  (a: array elt)
+  (#x1: Seq.seq elt) (p1: P.perm)
+  (#x2: Seq.seq elt) (p2: P.perm)
+: SteelGhost unit opened
+    (pts_to a p1 x1 `star` pts_to a p2 x2)
+    (fun _ -> pts_to a (p1 `P.sum_perm` p2) x1)
+    (fun _ -> True)
+    (fun _ _ _ -> x1 == x2)
+
+/// Reading the i-th element of an array a.
+/// TODO: we should also provide an atomic version for small types.
+[@@noextract_to "krml"] // primitive
+val index
+  (#t: Type) (#p: P.perm)
+  (a: array t)
+  (#s: Ghost.erased (Seq.seq t))
+  (i: U32.t)
+: Steel t
+    (pts_to a p s)
+    (fun _ -> pts_to a p s)
+    (fun _ -> U32.v i < length a)
+    (fun _ res _ -> U32.v i < Seq.length s /\ res == Seq.index s (U32.v i))
+
+/// Writing the value v at the i-th element of an array a.
+/// TODO: we should also provide an atomic version for small types.
+[@@noextract_to "krml"]
+val upd
+  (#t: Type)
+  (a: array t)
+  (s: Ghost.erased (Seq.seq t))
+  (i: U32.t)
+  (sq: squash (U32.v i < Seq.length s))
+  (v: t)
+: SteelT unit
+    (pts_to a P.full_perm s)
+    (fun res -> pts_to a P.full_perm (Seq.upd s (U32.v i) v))
+
+/// An array a1 is adjacent to an array a2 if and only if they have
+/// the same base array and the end of a1 coincides with the beginning
+/// of a2
+let adjacent (#elt: Type) (a1 a2: array elt) : Tot prop =
+  base (ptr_of a1) == base (ptr_of a2) /\
+  offset (ptr_of a1) + (length a1) == offset (ptr_of a2)
+
+/// If two arrays are adjacent, then we can compute their merge, with
+/// their combined lengths. By virtue of the length being ghost,
+/// Karamel will extract it as "let y = a1"
+inline_for_extraction
+[@@noextract_to "krml"]
+let merge (#elt: Type) (a1: array elt) (a2: Ghost.erased (array elt))
+: Pure (array elt)
+  (requires (adjacent a1 a2))
+  (ensures (fun y -> length y == length a1 + length a2))
+= (| ptr_of a1, Ghost.hide (length a1 + length a2) |)
+
+/// Adjacency and merging are associative.
+let merge_assoc (#elt: Type) (a1 a2 a3: array elt) : Lemma
+  (requires (adjacent a1 a2 /\ adjacent a2 a3))
+  (ensures (
+    adjacent (merge a1 a2) a3 /\ adjacent a1 (merge a2 a3) /\
+    merge (merge a1 a2) a3 == merge a1 (merge a2 a3)
+  ))
+= ()
+
+/// A shortcut to combine adjacency and merging
+let merge_into (#elt: Type) (a1 a2 a: array elt) : Tot prop =
+  adjacent a1 a2 /\
+  merge a1 a2 == a
+
+/// Spatial merging of two arrays, expressed in terms of `merge`.
+val ghost_join
+  (#opened: _)
+  (#elt: Type)
+  (#x1 #x2: Seq.seq elt)
+  (#p: P.perm)
+  (a1 a2: array elt)
+  (h: squash (adjacent a1 a2))
+: SteelGhostT unit opened
+    (pts_to a1 p x1 `star` pts_to a2 p x2)
+    (fun res -> pts_to (merge a1 a2) p (x1 `Seq.append` x2))
+
+/// Spatial merging, combining the use of `merge` and the call to the
+/// stateful lemma. Since the only operations are calls to stateful
+/// lemmas and pure computations, the overall computation is atomic
+/// and unobservable, so can be used anywhere in atomic contexts.  By
+/// virtue of the length being ghost, Karamel will extract this to
+/// "let res = a1"
+inline_for_extraction // this will extract to "let res = a1"
+[@@noextract_to "krml"]
+let join
+  (#opened: _)
+  (#elt: Type)
+  (#x1 #x2: Ghost.erased (Seq.seq elt))
+  (#p: P.perm)
+  (a1: array elt)
+  (a2: Ghost.erased (array elt))
+: SteelAtomicBase (array elt) false opened Unobservable
+    (pts_to a1 p x1 `star` pts_to a2 p x2)
+    (fun res -> pts_to res p (x1 `Seq.append` x2))
+    (fun _ -> adjacent a1 a2)
+    (fun _ res _ -> merge_into a1 a2 res)
+= ghost_join a1 a2 ();
+  let res = merge a1 a2 in
+  change_equal_slprop
+    (pts_to (merge a1 (Ghost.reveal a2)) p (x1 `Seq.append` x2))
+    (pts_to res p (x1 `Seq.append` x2));
+  return res
+
+/// Computing the left-hand-side part of splitting an array a at
+/// offset i.  By virtue of the length being ghost, Karamel will
+/// extract this to "let y = a"
+inline_for_extraction // this will extract to "let y = a"
+[@@noextract_to "krml"]
+let split_l (#elt: Type) (a: array elt)
+  (i: Ghost.erased U32.t)
+: Pure (array elt)
+  (requires (U32.v i <= length a))
+  (ensures (fun y -> True))
+= (| ptr_of a, Ghost.hide (U32.v i) |)
+
+/// C pointer arithmetic to compute (p+off), shifting a pointer p by
+/// offset off.  TODO: replace this with a Ghost definition and a
+/// SteelAtomicBase Unobservable operation with the corresponding
+/// permission.
+[@@noextract_to "krml"]
+val ptr_shift
+  (#elt: Type)
+  (p: ptr elt)
+  (off: U32.t)
+: Pure (ptr elt)
+  (requires (offset p + U32.v off <= base_len (base p)))
+  (ensures (fun p' ->
+    base p' == base p /\
+    offset p' == offset p + U32.v off
+  ))
+
+/// Computing the right-hand-side part of splitting an array a at
+/// offset i.
+inline_for_extraction
+[@@noextract_to "krml"]
+let split_r (#elt: Type) (a: array elt)
+  (i: U32.t)
+: Pure (array elt)
+  (requires (U32.v i <= length a))
+  (ensures (fun y -> merge_into (split_l a i) y a))
+= (| ptr_shift (ptr_of a) i, Ghost.hide (length a - U32.v i) |)
+
+/// Splitting an array a at offset i, as a stateful lemma expressed in
+/// terms of split_l, split_r. This stateful lemma returns a proof
+/// that offset i is in bounds of the value sequence, which is needed to
+/// typecheck the post-resource.
+val ghost_split
+  (#opened: _)
+  (#elt: Type)
+  (#x: Seq.seq elt)
+  (#p: P.perm)
+  (a: array elt)
+  (i: U32.t)
+: SteelGhost (squash (U32.v i <= length a /\ U32.v i <= Seq.length x)) opened
+    (pts_to a p x)
+    (fun res ->
+      pts_to (split_l a i) p (Seq.slice x 0 (U32.v i)) `star`
+      pts_to (split_r a i) p (Seq.slice x (U32.v i) (Seq.length x)))
+    (fun _ -> U32.v i <= length a)
+    (fun _ res _ ->
+      x == Seq.append (Seq.slice x 0 (U32.v i)) (Seq.slice x (U32.v i) (Seq.length x))
+    )
+
+/// NOTE: we could implement a SteelAtomicBase Unobservable "split"
+/// operation, just like "join", but we don't want it to return a pair
+/// of arrays. For now we settle on explicit use of split_l, split_r.
